

Steepest Descent

①

$$f(x) = \frac{1}{2} x^T Q x - b^T x$$

$$\text{where } x = \begin{bmatrix} x \\ y \end{bmatrix} \quad b = \begin{bmatrix} b_1 \\ b_2 \end{bmatrix} \quad Q = \begin{bmatrix} a & c \\ c & b \end{bmatrix}$$

$$f(x, y) = \frac{1}{2} \begin{bmatrix} x & y \end{bmatrix} \begin{bmatrix} a & c \\ c & b \end{bmatrix} \begin{bmatrix} x \\ y \end{bmatrix} - \begin{bmatrix} b_1 & b_2 \end{bmatrix} \begin{bmatrix} x \\ y \end{bmatrix}$$

$$\begin{aligned} f(x, y) &= \frac{1}{2} \begin{bmatrix} ax+cy & cx+by \end{bmatrix} \begin{bmatrix} x \\ y \end{bmatrix} - [b_1 x + b_2 y] \\ &= \frac{1}{2} [ax^2 + (cx+cy)y + by^2] - [b_1 x + b_2 y] \end{aligned}$$

$$\boxed{f(x, y) = \frac{a}{2} x^2 + cxy + \frac{b}{2} y^2 - b_1 x - b_2 y}$$

$$\nabla f(x) = \begin{pmatrix} \frac{\partial f}{\partial x} \\ \frac{\partial f}{\partial y} \end{pmatrix} = \begin{pmatrix} ax + cy - b_1 \\ cx + by - b_2 \end{pmatrix}$$

$$= \begin{pmatrix} a & c \\ c & b \end{pmatrix} \begin{pmatrix} x \\ y \end{pmatrix} - \begin{pmatrix} b_1 \\ b_2 \end{pmatrix}$$

$$= Qx - b$$

$$\nabla f(x) = -(b - Qx)$$

$$\{\nabla f(x)\}^T = [-(b - Qx)]^T$$

$$= -[b^T - x^T Q^T]$$

$$\{\nabla f(x)\}^T = -[b^T - x^T Q] \quad \text{since } Q = Q^T$$

$$-\{\nabla f(x)\}^T = b^T - x^T Q$$

Iterative procedure.

$$x_{k+1} = x_k - \eta_k \nabla f(x_k)$$

where η_k is the step size

$$\nabla f(x_k) = S, \quad Q = \begin{bmatrix} f_{xx} & f_{xy} \\ f_{yx} & f_{yy} \end{bmatrix} = \begin{bmatrix} a & c \\ c & b \end{bmatrix}$$

Derivation of η_k

$$\begin{aligned} g(\eta_k) &= f(x_{k+1}) \\ &= f(x_k - \eta_k \nabla f(x_k)) \\ &= \frac{1}{2} [x_k - \eta_k \nabla f(x_k)]^T Q [x_k - \eta_k \nabla f(x_k)] - b^T [x_k - \eta_k \nabla f(x_k)] \\ &= \frac{1}{2} x_k^T Q x_k - \frac{1}{2} (\eta_k \{\nabla f(x_k)\}^T Q x_k) - \frac{1}{2} (\eta_k x_k^T Q \nabla f(x_k)) \quad \text{same} \\ &\quad + \frac{1}{2} \{\nabla f(x_k)\}^T Q \nabla f(x_k) \eta_k^2 - b^T x_k + b^T \eta_k \nabla f(x_k) \\ &= \frac{1}{2} \{\nabla f(x_k)\}^T Q \nabla f(x_k) \eta_k^2 + b^T \nabla f(x_k) \eta_k - x_k^T Q \nabla f(x_k) \eta_k \\ &\quad + \frac{1}{2} x_k^T Q x_k - b^T x_k \\ &= \frac{1}{2} \{\nabla f(x_k)\}^T Q \nabla f(x_k) \eta_k^2 + (b^T - x_k^T Q) \nabla f(x_k) \eta_k \\ &\quad + \frac{1}{2} x_k^T Q x_k - b^T x_k \\ &= \frac{1}{2} \{\nabla f(x_k)\}^T Q \nabla f(x_k) \eta_k^2 + \left[-\{\nabla f(x_k)\}^T \right] \nabla f(x_k) \eta_k \\ &\quad + \frac{1}{2} x_k^T Q x_k - b^T x_k \end{aligned}$$

$$g(\eta_k) = A \eta_k^2 + B \eta_k + C$$

where

$$\begin{aligned} A &= \frac{1}{2} \{\nabla f(x_k)\}^T Q \nabla f(x_k) \\ B &= -\{\nabla f(x_k)\}^T \nabla f(x_k) \\ C &= \frac{1}{2} x_k^T Q x_k - b^T x_k. \end{aligned}$$

$$g(\eta_k) = A\eta_k^2 + B\eta_k + C \quad (2)$$

$$\frac{dg}{d\eta_k} = 2A\eta_k + B$$

Equate to zero $\frac{dg}{d\eta_k}$ for finding step size.

$$2A\eta_k + B = 0$$

$$\eta_k = \frac{-B}{2A}$$

$$\begin{aligned} &= \frac{\{\nabla f(x_k)\}^T \nabla f(x_k)}{\{\nabla f(x_k)\}^T Q \nabla f(x_k)} \\ &= \frac{S^T S}{S^T Q S} \end{aligned}$$

Where $S = \nabla f(x_k) = \begin{bmatrix} \frac{\partial f}{\partial x} \\ \frac{\partial f}{\partial y} \end{bmatrix}$

$Q = \begin{bmatrix} f_{xx} & f_{xy} \\ f_{yx} & f_{yy} \end{bmatrix}$ is Hessian matrix